Implement the scalar_tac_simp attribute

backends/lean/Aeneas/ScalarTac/ScalarTac.lean
@@ -8,9 +8,9 @@ namespace Std
 
 set_option maxRecDepth 1024
 
-theorem UScalar.max_USize_eq : UScalar.max .Usize = Usize.max := by rfl
-theorem IScalar.min_ISize_eq : IScalar.min .Isize = Isize.min := by rfl
-theorem IScalar.max_ISize_eq : IScalar.max .Isize = Isize.max := by rfl
+@[scalar_tac_simp] theorem UScalar.max_USize_eq : UScalar.max .Usize = Usize.max := by rfl
+@[scalar_tac_simp] theorem IScalar.min_ISize_eq : IScalar.min .Isize = Isize.min := by rfl
+@[scalar_tac_simp] theorem IScalar.max_ISize_eq : IScalar.max .Isize = Isize.max := by rfl
 
 theorem Usize.max_succ_eq_pow : Usize.max + 1 = 2^System.Platform.numBits := by
   simp [Usize.max, Usize.numBits]
@@ -38,97 +38,99 @@ theorem Isize.cMin_cMax_bound : Isize.min ≤ IScalar.cMin .Isize ∧ IScalar.cM
         Isize.max, IScalar.cMax, IScalar.rMax, I32.rMax]
   have := System.Platform.numBits_eq; cases this <;> simp [*]
 
-def U8.numBits_eq    : U8.numBits = 8 := by rfl
-def U16.numBits_eq   : U16.numBits = 16 := by rfl
-def U32.numBits_eq   : U32.numBits = 32 := by rfl
-def U64.numBits_eq   : U64.numBits = 64 := by rfl
-def U128.numBits_eq  : U128.numBits = 128 := by rfl
-def Usize.numBits_eq : Usize.numBits = System.Platform.numBits := by rfl
+@[scalar_tac_simp] theorem U8.numBits_eq    : U8.numBits = 8 := by rfl
+@[scalar_tac_simp] theorem U16.numBits_eq   : U16.numBits = 16 := by rfl
+@[scalar_tac_simp] theorem U32.numBits_eq   : U32.numBits = 32 := by rfl
+@[scalar_tac_simp] theorem U64.numBits_eq   : U64.numBits = 64 := by rfl
+@[scalar_tac_simp] theorem U128.numBits_eq  : U128.numBits = 128 := by rfl
+@[scalar_tac_simp] theorem Usize.numBits_eq : Usize.numBits = System.Platform.numBits := by rfl
 
-def I8.numBits_eq    : I8.numBits = 8 := by rfl
-def I16.numBits_eq   : I16.numBits = 16 := by rfl
-def I32.numBits_eq   : I32.numBits = 32 := by rfl
-def I64.numBits_eq   : I64.numBits = 64 := by rfl
-def I128.numBits_eq  : I128.numBits = 128 := by rfl
-def Isize.numBits_eq : Isize.numBits = System.Platform.numBits := by rfl
+@[scalar_tac_simp] theorem I8.numBits_eq    : I8.numBits = 8 := by rfl
+@[scalar_tac_simp] theorem I16.numBits_eq   : I16.numBits = 16 := by rfl
+@[scalar_tac_simp] theorem I32.numBits_eq   : I32.numBits = 32 := by rfl
+@[scalar_tac_simp] theorem I64.numBits_eq   : I64.numBits = 64 := by rfl
+@[scalar_tac_simp] theorem I128.numBits_eq  : I128.numBits = 128 := by rfl
+@[scalar_tac_simp] theorem Isize.numBits_eq : Isize.numBits = System.Platform.numBits := by rfl
 
-theorem U8.max_eq    : U8.max = 255 := by rfl
-theorem U16.max_eq   : U16.max = 65535 := by rfl
-theorem U32.max_eq   : U32.max = 4294967295 := by rfl
-theorem U64.max_eq   : U64.max = 18446744073709551615 := by rfl
-theorem U128.max_eq  : U128.max = 340282366920938463463374607431768211455 := by rfl
+@[scalar_tac_simp] theorem U8.max_eq    : U8.max = 255 := by rfl
+@[scalar_tac_simp] theorem U16.max_eq   : U16.max = 65535 := by rfl
+@[scalar_tac_simp] theorem U32.max_eq   : U32.max = 4294967295 := by rfl
+@[scalar_tac_simp] theorem U64.max_eq   : U64.max = 18446744073709551615 := by rfl
+@[scalar_tac_simp] theorem U128.max_eq  : U128.max = 340282366920938463463374607431768211455 := by rfl
 
-theorem UScalar.max_U8_eq    : UScalar.max .U8 = 255 := by rfl
-theorem UScalar.max_U16_eq   : UScalar.max .U16 = 65535 := by rfl
-theorem UScalar.max_U32_eq   : UScalar.max .U32 = 4294967295 := by rfl
-theorem UScalar.max_U64_eq   : UScalar.max .U64 = 18446744073709551615 := by rfl
-theorem UScalar.max_U128_eq  : UScalar.max .U128 = 340282366920938463463374607431768211455 := by rfl
+@[scalar_tac_simp] theorem UScalar.max_U8_eq    : UScalar.max .U8 = 255 := by rfl
+@[scalar_tac_simp] theorem UScalar.max_U16_eq   : UScalar.max .U16 = 65535 := by rfl
+@[scalar_tac_simp] theorem UScalar.max_U32_eq   : UScalar.max .U32 = 4294967295 := by rfl
+@[scalar_tac_simp] theorem UScalar.max_U64_eq   : UScalar.max .U64 = 18446744073709551615 := by rfl
+@[scalar_tac_simp] theorem UScalar.max_U128_eq  : UScalar.max .U128 = 340282366920938463463374607431768211455 := by rfl
 
-theorem I8.min_eq    : I8.min = -128 := by rfl
-theorem I8.max_eq    : I8.max = 127 := by rfl
-theorem I16.min_eq   : I16.min = -32768 := by rfl
-theorem I16.max_eq   : I16.max = 32767 := by rfl
-theorem I32.min_eq   : I32.min = -2147483648 := by rfl
-theorem I32.max_eq   : I32.max = 2147483647 := by rfl
-theorem I64.min_eq   : I64.min = -9223372036854775808 := by rfl
-theorem I64.max_eq   : I64.max = 9223372036854775807 := by rfl
-theorem I128.min_eq  : I128.min = -170141183460469231731687303715884105728 := by rfl
-theorem I128.max_eq  : I128.max = 170141183460469231731687303715884105727 := by rfl
+@[scalar_tac_simp] theorem I8.min_eq    : I8.min = -128 := by rfl
+@[scalar_tac_simp] theorem I8.max_eq    : I8.max = 127 := by rfl
+@[scalar_tac_simp] theorem I16.min_eq   : I16.min = -32768 := by rfl
+@[scalar_tac_simp] theorem I16.max_eq   : I16.max = 32767 := by rfl
+@[scalar_tac_simp] theorem I32.min_eq   : I32.min = -2147483648 := by rfl
+@[scalar_tac_simp] theorem I32.max_eq   : I32.max = 2147483647 := by rfl
+@[scalar_tac_simp] theorem I64.min_eq   : I64.min = -9223372036854775808 := by rfl
+@[scalar_tac_simp] theorem I64.max_eq   : I64.max = 9223372036854775807 := by rfl
+@[scalar_tac_simp] theorem I128.min_eq  : I128.min = -170141183460469231731687303715884105728 := by rfl
+@[scalar_tac_simp] theorem I128.max_eq  : I128.max = 170141183460469231731687303715884105727 := by rfl
 
-theorem IScalar.min_I8_eq    : IScalar.min .I8 = -128 := by rfl
-theorem IScalar.max_I8_eq    : IScalar.max .I8 = 127 := by rfl
-theorem IScalar.min_I16_eq   : IScalar.min .I16 = -32768 := by rfl
-theorem IScalar.max_I16_eq   : IScalar.max .I16 = 32767 := by rfl
-theorem IScalar.min_I32_eq   : IScalar.min .I32 = -2147483648 := by rfl
-theorem IScalar.max_I32_eq   : IScalar.max .I32 = 2147483647 := by rfl
-theorem IScalar.min_I64_eq   : IScalar.min .I64 = -9223372036854775808 := by rfl
-theorem IScalar.max_I64_eq   : IScalar.max .I64 = 9223372036854775807 := by rfl
-theorem IScalar.min_I128_eq  : IScalar.min .I128 = -170141183460469231731687303715884105728 := by rfl
-theorem IScalar.max_I128_eq  : IScalar.max .I128 = 170141183460469231731687303715884105727 := by rfl
+@[scalar_tac_simp] theorem IScalar.min_I8_eq    : IScalar.min .I8 = -128 := by rfl
+@[scalar_tac_simp] theorem IScalar.max_I8_eq    : IScalar.max .I8 = 127 := by rfl
+@[scalar_tac_simp] theorem IScalar.min_I16_eq   : IScalar.min .I16 = -32768 := by rfl
+@[scalar_tac_simp] theorem IScalar.max_I16_eq   : IScalar.max .I16 = 32767 := by rfl
+@[scalar_tac_simp] theorem IScalar.min_I32_eq   : IScalar.min .I32 = -2147483648 := by rfl
+@[scalar_tac_simp] theorem IScalar.max_I32_eq   : IScalar.max .I32 = 2147483647 := by rfl
+@[scalar_tac_simp] theorem IScalar.min_I64_eq   : IScalar.min .I64 = -9223372036854775808 := by rfl
+@[scalar_tac_simp] theorem IScalar.max_I64_eq   : IScalar.max .I64 = 9223372036854775807 := by rfl
+@[scalar_tac_simp] theorem IScalar.min_I128_eq  : IScalar.min .I128 = -170141183460469231731687303715884105728 := by rfl
+@[scalar_tac_simp] theorem IScalar.max_I128_eq  : IScalar.max .I128 = 170141183460469231731687303715884105727 := by rfl
 
-theorem U8.size_eq    : U8.size = 256 := by rfl
-theorem U16.size_eq   : U16.size = 65536 := by rfl
-theorem U32.size_eq   : U32.size = 4294967296 := by rfl
-theorem U64.size_eq   : U64.size = 18446744073709551616 := by rfl
-theorem U128.size_eq  : U128.size = 340282366920938463463374607431768211456 := by rfl
+@[scalar_tac_simp] theorem U8.size_eq    : U8.size = 256 := by rfl
+@[scalar_tac_simp] theorem U16.size_eq   : U16.size = 65536 := by rfl
+@[scalar_tac_simp] theorem U32.size_eq   : U32.size = 4294967296 := by rfl
+@[scalar_tac_simp] theorem U64.size_eq   : U64.size = 18446744073709551616 := by rfl
+@[scalar_tac_simp] theorem U128.size_eq  : U128.size = 340282366920938463463374607431768211456 := by rfl
 
-theorem I8.size_eq    : I8.size = 256 := by rfl
-theorem I16.size_eq   : I16.size = 65536 := by rfl
-theorem I32.size_eq   : I32.size = 4294967296 := by rfl
-theorem I64.size_eq   : I64.size = 18446744073709551616 := by rfl
-theorem I128.size_eq  : I128.size = 340282366920938463463374607431768211456 := by rfl
+@[scalar_tac_simp] theorem I8.size_eq    : I8.size = 256 := by rfl
+@[scalar_tac_simp] theorem I16.size_eq   : I16.size = 65536 := by rfl
+@[scalar_tac_simp] theorem I32.size_eq   : I32.size = 4294967296 := by rfl
+@[scalar_tac_simp] theorem I64.size_eq   : I64.size = 18446744073709551616 := by rfl
+@[scalar_tac_simp] theorem I128.size_eq  : I128.size = 340282366920938463463374607431768211456 := by rfl
 
-theorem UScalar.size_U8_eq    : UScalar.size .U8 = 256 := by rfl
-theorem UScalar.size_U16_eq   : U16.size = 65536 := by rfl
-theorem UScalar.size_U32_eq   : UScalar.size .U32 = 4294967296 := by rfl
-theorem UScalar.size_U64_eq   : UScalar.size .U64 = 18446744073709551616 := by rfl
-theorem UScalar.size_U128_eq  : UScalar.size .U128 = 340282366920938463463374607431768211456 := by rfl
+@[scalar_tac_simp] theorem UScalar.size_U8_eq    : UScalar.size .U8 = 256 := by rfl
+@[scalar_tac_simp] theorem UScalar.size_U16_eq   : U16.size = 65536 := by rfl
+@[scalar_tac_simp] theorem UScalar.size_U32_eq   : UScalar.size .U32 = 4294967296 := by rfl
+@[scalar_tac_simp] theorem UScalar.size_U64_eq   : UScalar.size .U64 = 18446744073709551616 := by rfl
+@[scalar_tac_simp] theorem UScalar.size_U128_eq  : UScalar.size .U128 = 340282366920938463463374607431768211456 := by rfl
 
-theorem IScalar.size_I8_eq    : IScalar.size .I8 = 256 := by rfl
-theorem IScalar.size_I16_eq   : IScalar.size .I16 = 65536 := by rfl
-theorem IScalar.size_I32_eq   : IScalar.size .I32 = 4294967296 := by rfl
-theorem IScalar.size_I64_eq   : IScalar.size .I64 = 18446744073709551616 := by rfl
-theorem IScalar.size_I128_eq  : IScalar.size .I128 = 340282366920938463463374607431768211456 := by rfl
+@[scalar_tac_simp] theorem IScalar.size_I8_eq    : IScalar.size .I8 = 256 := by rfl
+@[scalar_tac_simp] theorem IScalar.size_I16_eq   : IScalar.size .I16 = 65536 := by rfl
+@[scalar_tac_simp] theorem IScalar.size_I32_eq   : IScalar.size .I32 = 4294967296 := by rfl
+@[scalar_tac_simp] theorem IScalar.size_I64_eq   : IScalar.size .I64 = 18446744073709551616 := by rfl
+@[scalar_tac_simp] theorem IScalar.size_I128_eq  : IScalar.size .I128 = 340282366920938463463374607431768211456 := by rfl
 
-theorem UScalar.cMax_U8_eq     : UScalar.cMax .U8 = 255 := by rfl
-theorem UScalar.cMax_U16_eq    : UScalar.cMax .U16 = 65535 := by rfl
-theorem UScalar.cMax_U32_eq    : UScalar.cMax .U32 = 4294967295 := by rfl
-theorem UScalar.cMax_U64_eq    : UScalar.cMax .U64 = 18446744073709551615 := by rfl
-theorem UScalar.cMax_U128_eq   : UScalar.cMax .U128 = 340282366920938463463374607431768211455 := by rfl
-theorem UScalar.cMax_Usize_eq  : UScalar.cMax .Usize = 4294967295 := by rfl
+@[scalar_tac_simp] theorem UScalar.cMax_U8_eq     : UScalar.cMax .U8 = 255 := by rfl
+@[scalar_tac_simp] theorem UScalar.cMax_U16_eq    : UScalar.cMax .U16 = 65535 := by rfl
+@[scalar_tac_simp] theorem UScalar.cMax_U32_eq    : UScalar.cMax .U32 = 4294967295 := by rfl
+@[scalar_tac_simp] theorem UScalar.cMax_U64_eq    : UScalar.cMax .U64 = 18446744073709551615 := by rfl
+@[scalar_tac_simp] theorem UScalar.cMax_U128_eq   : UScalar.cMax .U128 = 340282366920938463463374607431768211455 := by rfl
+@[scalar_tac_simp] theorem UScalar.cMax_Usize_eq  : UScalar.cMax .Usize = 4294967295 := by rfl
 
-theorem IScalar.cMin_I8_eq     : IScalar.cMin .I8 = -128 := by rfl
-theorem IScalar.cMax_I8_eq     : IScalar.cMax .I8 = 127 := by rfl
-theorem IScalar.cMin_I16_eq    : IScalar.cMin .I16 = -32768 := by rfl
-theorem IScalar.cMax_I16_eq    : IScalar.cMax .I16 = 32767 := by rfl
-theorem IScalar.cMin_I32_eq    : IScalar.cMin .I32 = -2147483648 := by rfl
-theorem IScalar.cMax_I32_eq    : IScalar.cMax .I32 = 2147483647 := by rfl
-theorem IScalar.cMin_I64_eq    : IScalar.cMin .I64 = -9223372036854775808 := by rfl
-theorem IScalar.cMax_I64_eq    : IScalar.cMax .I64 = 9223372036854775807 := by rfl
-theorem IScalar.cMin_I128_eq   : IScalar.cMin .I128 = -170141183460469231731687303715884105728 := by rfl
-theorem IScalar.cMax_I128_eq   : IScalar.cMax .I128 = 170141183460469231731687303715884105727 := by rfl
-theorem IScalar.cMin_Isize_eq  : IScalar.cMin .Isize = -2147483648 := by rfl
-theorem IScalar.cMax_Isize_eq  : IScalar.cMax .Isize = 2147483647 := by rfl
+@[scalar_tac_simp] theorem IScalar.cMin_I8_eq     : IScalar.cMin .I8 = -128 := by rfl
+@[scalar_tac_simp] theorem IScalar.cMax_I8_eq     : IScalar.cMax .I8 = 127 := by rfl
+@[scalar_tac_simp] theorem IScalar.cMin_I16_eq    : IScalar.cMin .I16 = -32768 := by rfl
+@[scalar_tac_simp] theorem IScalar.cMax_I16_eq    : IScalar.cMax .I16 = 32767 := by rfl
+@[scalar_tac_simp] theorem IScalar.cMin_I32_eq    : IScalar.cMin .I32 = -2147483648 := by rfl
+@[scalar_tac_simp] theorem IScalar.cMax_I32_eq    : IScalar.cMax .I32 = 2147483647 := by rfl
+@[scalar_tac_simp] theorem IScalar.cMin_I64_eq    : IScalar.cMin .I64 = -9223372036854775808 := by rfl
+@[scalar_tac_simp] theorem IScalar.cMax_I64_eq    : IScalar.cMax .I64 = 9223372036854775807 := by rfl
+@[scalar_tac_simp] theorem IScalar.cMin_I128_eq   : IScalar.cMin .I128 = -170141183460469231731687303715884105728 := by rfl
+@[scalar_tac_simp] theorem IScalar.cMax_I128_eq   : IScalar.cMax .I128 = 170141183460469231731687303715884105727 := by rfl
+@[scalar_tac_simp] theorem IScalar.cMin_Isize_eq  : IScalar.cMin .Isize = -2147483648 := by rfl
+@[scalar_tac_simp] theorem IScalar.cMax_Isize_eq  : IScalar.cMax .Isize = 2147483647 := by rfl
+
+attribute [scalar_tac_simp] Bool.toNat_false Bool.toNat_true
 
 end Std
 
@@ -138,48 +140,20 @@ namespace ScalarTac
 open Lean Lean.Elab Lean.Meta
 open Std
 
-def scalarTacSimpLemmas := [
-  ``UScalar.ofNat_val_eq, ``UScalar.neq_to_neq_val,
-  ``IScalar.ofInt_val_eq, ``IScalar.neq_to_neq_val,
-  ``UScalar.bv_toNat_eq,
-  ``U8.bv_toNat_eq, ``U16.bv_toNat_eq, ``U32.bv_toNat_eq, ``U64.bv_toNat_eq, ``U128.bv_toNat_eq, ``Usize.bv_toNat_eq,
-  ``IScalar.bv_toInt_eq,
-  ``I8.bv_toInt_eq, ``I16.bv_toInt_eq, ``I32.bv_toInt_eq, ``I64.bv_toInt_eq, ``I128.bv_toInt_eq, ``Isize.bv_toInt_eq,
-  ``UScalar.lt_equiv, ``UScalar.le_equiv, ``UScalar.eq_equiv,
-  ``IScalar.lt_equiv, ``IScalar.le_equiv, ``IScalar.eq_equiv,
-  ``U8.ofNat_val_eq, ``U16.ofNat_val_eq, ``U32.ofNat_val_eq, ``U64.ofNat_val_eq, ``U128.ofNat_val_eq, ``Usize.ofNat_val_eq,
-  ``UScalarTy.U8_numBits_eq, ``UScalarTy.U16_numBits_eq, ``UScalarTy.U32_numBits_eq, ``UScalarTy.U64_numBits_eq, ``UScalarTy.U128_numBits_eq, ``UScalarTy.Usize_numBits_eq,
-  ``IScalarTy.I8_numBits_eq, ``IScalarTy.I16_numBits_eq, ``IScalarTy.I32_numBits_eq, ``IScalarTy.I64_numBits_eq, ``IScalarTy.I128_numBits_eq, ``IScalarTy.Isize_numBits_eq,
-  ``U8.numBits_eq, ``U16.numBits_eq, ``U32.numBits_eq, ``U64.numBits_eq, ``U128.numBits_eq, ``Usize.numBits_eq,
-  ``I8.numBits_eq, ``I16.numBits_eq, ``I32.numBits_eq, ``I64.numBits_eq, ``I128.numBits_eq, ``Isize.numBits_eq,
-  ``UScalar.max_USize_eq, ``IScalar.min_ISize_eq, ``IScalar.max_ISize_eq,
-  ``UScalar.cMax_U8_eq, ``UScalar.cMax_U16_eq, ``UScalar.cMax_U32_eq, ``UScalar.cMax_U64_eq, ``UScalar.cMax_U128_eq, ``UScalar.cMax_Usize_eq,
-  ``IScalar.cMin_I8_eq, ``IScalar.cMin_I16_eq, ``IScalar.cMin_I32_eq, ``IScalar.cMin_I64_eq, ``IScalar.cMin_I128_eq, ``IScalar.cMin_Isize_eq,
-  ``IScalar.cMax_I8_eq, ``IScalar.cMax_I16_eq, ``IScalar.cMax_I32_eq, ``IScalar.cMax_I64_eq, ``IScalar.cMax_I128_eq, ``IScalar.cMax_Isize_eq,
-  ``UScalar.max_U8_eq, ``UScalar.max_U16_eq, ``UScalar.max_U32_eq, ``UScalar.max_U64_eq, ``UScalar.max_U128_eq,
-  ``IScalar.min_I8_eq, ``IScalar.min_I16_eq, ``IScalar.min_I32_eq, ``IScalar.min_I64_eq, ``IScalar.min_I128_eq,
-  ``IScalar.max_I8_eq, ``IScalar.max_I16_eq, ``IScalar.max_I32_eq, ``IScalar.max_I64_eq, ``IScalar.max_I128_eq,
-  ``UScalar.size_U8_eq, ``UScalar.size_U16_eq, ``UScalar.size_U32_eq, ``UScalar.size_U64_eq, ``UScalar.size_U128_eq,
-  ``IScalar.size_I8_eq, ``IScalar.size_I16_eq, ``IScalar.size_I32_eq, ``IScalar.size_I64_eq, ``IScalar.size_I128_eq,
-  ``U8.max_eq, ``U16.max_eq, ``U32.max_eq, ``U64.max_eq, ``U128.max_eq,
-  ``I8.min_eq, ``I16.min_eq, ``I32.min_eq, ``I64.min_eq, ``I128.min_eq,
-  ``I8.max_eq, ``I16.max_eq, ``I32.max_eq, ``I64.max_eq, ``I128.max_eq,
-  ``U8.size_eq, ``U16.size_eq, ``U32.size_eq, ``U64.size_eq, ``U128.size_eq,
-  ``I8.size_eq, ``I16.size_eq, ``I32.size_eq, ``I64.size_eq, ``I128.size_eq,
-  ``Bool.toNat_false, ``Bool.toNat_true
-  ]
-
 def scalarTacExtraPrePreprocess : Tactic.TacticM Unit :=
   Tactic.withMainContext do
   -- First get rid of [ofInt] (if there are dependent arguments, we may not
   -- manage to simplify the context)
+  let simpLemmas ← scalarTacSimpExt.getTheorems
   Utils.simpAt true {dsimp := false, failIfUnchanged := false}
-               -- Simprocs
-               intTacSimpRocs
-               -- Unfoldings
-               []
+                -- Simprocs
+                intTacSimpRocs
+                -- Simp theorems
+                [simpLemmas]
+                -- Unfoldings
+                []
                 -- Simp lemmas
-                scalarTacSimpLemmas
+                []
                 -- Hypotheses
                 [] .wildcard
 
@@ -192,13 +166,16 @@ def scalarTacExtraPreprocess : Tactic.TacticM Unit := do
   add (← mkAppM ``Usize.cMax_bound #[])
   add (← mkAppM ``Isize.cMin_cMax_bound #[])
   add (← mkAppM ``Usize_Isize_min_max_eqs #[])
+  let simpLemmas ← scalarTacSimpExt.getTheorems
   Utils.simpAt true {failIfUnchanged := false}
-               -- Simprocs
-               intTacSimpRocs
-               -- Unfoldings
-               [``Isize.toNat, ``I8.toNat, ``I16.toNat, ``I32.toNat, ``I64.toNat, ``I128.toNat]
+                -- Simprocs
+                intTacSimpRocs
+                -- Simp theorems
+                [simpLemmas]
+                -- Unfoldings
+                [``Isize.toNat, ``I8.toNat, ``I16.toNat, ``I32.toNat, ``I64.toNat, ``I128.toNat]
                 -- Simp lemmas
-                scalarTacSimpLemmas
+                []
                 -- Hypotheses
                 [] .wildcard
   trace[ScalarTac] "scalarTacExtraPreprocess: after simp: {(← Tactic.getMainGoal)}"
