backends/lean/Aeneas/Std/ScalarCore.lean
@@ -616,31 +616,31 @@ abbrev I32.ofInt   := @IScalar.ofInt .I32
 abbrev I64.ofInt   := @IScalar.ofInt .I64
 abbrev I128.ofInt  := @IScalar.ofInt .I128
 
-@[simp] theorem UScalar.ofNat_val_eq {ty : UScalarTy} (h : x < 2^ty.numBits) :
+@[simp, scalar_tac_simp] theorem UScalar.ofNat_val_eq {ty : UScalarTy} (h : x < 2^ty.numBits) :
   (UScalar.ofNatCore x h).val = x := by
   simp [UScalar.ofNat, UScalar.ofNatCore, UScalar.val, max]
   dcases ty <;> simp_all
   cases h: System.Platform.numBits_eq <;> simp_all
 
-@[simp] theorem U8.ofNat_val_eq (h : x < 2^U8.numBits) : (U8.ofNatCore x h).val = x := by
+@[simp, scalar_tac_simp] theorem U8.ofNat_val_eq (h : x < 2^U8.numBits) : (U8.ofNatCore x h).val = x := by
   apply UScalar.ofNat_val_eq h
 
-@[simp] theorem U16.ofNat_val_eq (h : x < 2^U16.numBits) : (U16.ofNatCore x h).val = x := by
+@[simp, scalar_tac_simp] theorem U16.ofNat_val_eq (h : x < 2^U16.numBits) : (U16.ofNatCore x h).val = x := by
   apply UScalar.ofNat_val_eq h
 
-@[simp] theorem U32.ofNat_val_eq (h : x < 2^U32.numBits) : (U32.ofNatCore x h).val = x := by
+@[simp, scalar_tac_simp] theorem U32.ofNat_val_eq (h : x < 2^U32.numBits) : (U32.ofNatCore x h).val = x := by
   apply UScalar.ofNat_val_eq h
 
-@[simp] theorem U64.ofNat_val_eq (h : x < 2^U64.numBits) : (U64.ofNatCore x h).val = x := by
+@[simp, scalar_tac_simp] theorem U64.ofNat_val_eq (h : x < 2^U64.numBits) : (U64.ofNatCore x h).val = x := by
   apply UScalar.ofNat_val_eq h
 
-@[simp] theorem U128.ofNat_val_eq (h : x < 2^U128.numBits) : (U128.ofNatCore x h).val = x := by
+@[simp, scalar_tac_simp] theorem U128.ofNat_val_eq (h : x < 2^U128.numBits) : (U128.ofNatCore x h).val = x := by
   apply UScalar.ofNat_val_eq h
 
-@[simp] theorem Usize.ofNat_val_eq (h : x < 2^Usize.numBits) : (Usize.ofNatCore x h).val = x := by
+@[simp, scalar_tac_simp] theorem Usize.ofNat_val_eq (h : x < 2^Usize.numBits) : (Usize.ofNatCore x h).val = x := by
   apply UScalar.ofNat_val_eq h
 
-@[simp] theorem IScalar.ofInt_val_eq {ty : IScalarTy} (h : - 2^(ty.numBits - 1) ≤ x ∧ x < 2^(ty.numBits - 1)) :
+@[simp, scalar_tac_simp] theorem IScalar.ofInt_val_eq {ty : IScalarTy} (h : - 2^(ty.numBits - 1) ≤ x ∧ x < 2^(ty.numBits - 1)) :
   (IScalar.ofIntCore x h).val = x := by
   simp [IScalar.ofInt, IScalar.ofIntCore, IScalar.val]
   dcases ty <;>
@@ -648,22 +648,22 @@ abbrev I128.ofInt  := @IScalar.ofInt .I128
   simp [Int.bmod] <;> split <;> (try omega) <;>
   cases h: System.Platform.numBits_eq <;> simp_all <;> omega
 
-@[simp] theorem I8.ofInt_val_eq (h : -2^(I8.numBits-1) ≤ x ∧ x < 2^(I8.numBits-1)) : (I8.ofIntCore x h).val = x := by
+@[simp, scalar_tac_simp] theorem I8.ofInt_val_eq (h : -2^(I8.numBits-1) ≤ x ∧ x < 2^(I8.numBits-1)) : (I8.ofIntCore x h).val = x := by
   apply IScalar.ofInt_val_eq
 
-@[simp] theorem I16.ofInt_val_eq (h : -2^(I16.numBits-1) ≤ x ∧ x < 2^(I16.numBits-1)) : (I16.ofIntCore x h).val = x := by
+@[simp, scalar_tac_simp] theorem I16.ofInt_val_eq (h : -2^(I16.numBits-1) ≤ x ∧ x < 2^(I16.numBits-1)) : (I16.ofIntCore x h).val = x := by
   apply IScalar.ofInt_val_eq
 
-@[simp] theorem I32.ofInt_val_eq (h : -2^(I32.numBits-1) ≤ x ∧ x < 2^(I32.numBits-1)) : (I32.ofIntCore x h).val = x := by
+@[simp, scalar_tac_simp] theorem I32.ofInt_val_eq (h : -2^(I32.numBits-1) ≤ x ∧ x < 2^(I32.numBits-1)) : (I32.ofIntCore x h).val = x := by
   apply IScalar.ofInt_val_eq
 
-@[simp] theorem I64.ofInt_val_eq (h : -2^(I64.numBits-1) ≤ x ∧ x < 2^(I64.numBits-1)) : (I64.ofIntCore x h).val = x := by
+@[simp, scalar_tac_simp] theorem I64.ofInt_val_eq (h : -2^(I64.numBits-1) ≤ x ∧ x < 2^(I64.numBits-1)) : (I64.ofIntCore x h).val = x := by
   apply IScalar.ofInt_val_eq
 
-@[simp] theorem I128.ofInt_val_eq (h : -2^(I128.numBits-1) ≤ x ∧ x < 2^(I128.numBits-1)) : (I128.ofIntCore x h).val = x := by
+@[simp, scalar_tac_simp] theorem I128.ofInt_val_eq (h : -2^(I128.numBits-1) ≤ x ∧ x < 2^(I128.numBits-1)) : (I128.ofIntCore x h).val = x := by
   apply IScalar.ofInt_val_eq
 
-@[simp] theorem Isize.ofInt_val_eq (h : -2^(Isize.numBits-1) ≤ x ∧ x < 2^(Isize.numBits-1)) : (Isize.ofIntCore x h).val = x := by
+@[simp, scalar_tac_simp] theorem Isize.ofInt_val_eq (h : -2^(Isize.numBits-1) ≤ x ∧ x < 2^(Isize.numBits-1)) : (Isize.ofIntCore x h).val = x := by
   apply IScalar.ofInt_val_eq
 
 instance (ty : UScalarTy) : Inhabited (UScalar ty) := by
@@ -721,28 +721,28 @@ instance {ty} : LE (IScalar ty) where le a b := LE.le a.val b.val
 
 /- Not marking this one with @[simp] on purpose: if we have `x = y` somewhere in the context,
    we may want to use it to substitute `y` with `x` somewhere. -/
-theorem UScalar.eq_equiv {ty : UScalarTy} (x y : UScalar ty) :
+@[scalar_tac_simp] theorem UScalar.eq_equiv {ty : UScalarTy} (x y : UScalar ty) :
   x = y ↔ (↑x : Nat) = ↑y := by
   cases x; cases y; simp_all [UScalar.val, BitVec.toNat_eq]
 
 @[simp] theorem UScalar.eq_imp {ty : UScalarTy} (x y : UScalar ty) :
   (↑x : Nat) = ↑y → x = y := (eq_equiv x y).mpr
 
-@[simp] theorem UScalar.lt_equiv {ty : UScalarTy} (x y : UScalar ty) :
+@[simp, scalar_tac_simp] theorem UScalar.lt_equiv {ty : UScalarTy} (x y : UScalar ty) :
   x < y ↔ (↑x : Nat) < ↑y := by
   rw [LT.lt, instLTUScalar]
 
 @[simp] theorem UScalar.lt_imp {ty : UScalarTy} (x y : UScalar ty) :
   (↑x : Nat) < (↑y) → x < y := (lt_equiv x y).mpr
 
-@[simp] theorem UScalar.le_equiv {ty : UScalarTy} (x y : UScalar ty) :
+@[simp, scalar_tac_simp] theorem UScalar.le_equiv {ty : UScalarTy} (x y : UScalar ty) :
   x ≤ y ↔ (↑x : Nat) ≤ ↑y := by
   rw [LE.le, instLEUScalar]
 
 @[simp] theorem UScalar.le_imp {ty : UScalarTy} (x y : UScalar ty) :
   (↑x : Nat) ≤ ↑y → x ≤ y := (le_equiv x y).mpr
 
-theorem IScalar.eq_equiv {ty : IScalarTy} (x y : IScalar ty) :
+@[scalar_tac_simp] theorem IScalar.eq_equiv {ty : IScalarTy} (x y : IScalar ty) :
   x = y ↔ (↑x : Int) = ↑y := by
   cases x; cases y; simp_all [IScalar.val]
   constructor <;> intro <;>
@@ -751,11 +751,11 @@ theorem IScalar.eq_equiv {ty : IScalarTy} (x y : IScalar ty) :
 @[simp] theorem IScalar.eq_imp {ty : IScalarTy} (x y : IScalar ty) :
   (↑x : Int) = ↑y → x = y := (eq_equiv x y).mpr
 
-@[simp] theorem IScalar.lt_equiv {ty : IScalarTy} (x y : IScalar ty) :
+@[simp, scalar_tac_simp] theorem IScalar.lt_equiv {ty : IScalarTy} (x y : IScalar ty) :
   x < y ↔ (↑x : Int) < ↑y := by
   rw [LT.lt, instLTIScalar]
 
-@[simp] theorem IScalar.lt_imp {ty : IScalarTy} (x y : IScalar ty) :
+@[simp, scalar_tac_simp] theorem IScalar.lt_imp {ty : IScalarTy} (x y : IScalar ty) :
   (↑x : Int) < (↑y) → x < y := (lt_equiv x y).mpr
 
 @[simp] theorem IScalar.le_equiv {ty : IScalarTy} (x y : IScalar ty) :
@@ -799,10 +799,10 @@ instance (ty : IScalarTy) : DecidableEq (IScalar ty) :=
     | isTrue h  => isTrue (IScalar.eq_of_val_eq h)
     | isFalse h => isFalse (IScalar.ne_of_val_ne h)
 
-@[simp] theorem UScalar.neq_to_neq_val {ty} : ∀ {i j : UScalar ty}, (¬ i = j) ↔ ¬ i.val = j.val := by
+@[simp, scalar_tac_simp] theorem UScalar.neq_to_neq_val {ty} : ∀ {i j : UScalar ty}, (¬ i = j) ↔ ¬ i.val = j.val := by
   simp [eq_equiv]
 
-@[simp] theorem IScalar.neq_to_neq_val {ty} : ∀ {i j : IScalar ty}, (¬ i = j) ↔ ¬ i.val = j.val := by
+@[simp, scalar_tac_simp] theorem IScalar.neq_to_neq_val {ty} : ∀ {i j : IScalar ty}, (¬ i = j) ↔ ¬ i.val = j.val := by
   simp [eq_equiv]
 
 @[simp]
@@ -920,27 +920,27 @@ def I64.bv (x : I64) : BitVec 64 := IScalar.bv x
 def I128.bv (x : I128) : BitVec 128 := IScalar.bv x
 def Isize.bv (x : Isize) : BitVec System.Platform.numBits := IScalar.bv x
 
-@[simp] theorem UScalar.bv_toNat_eq {ty : UScalarTy} (x : UScalar ty) :
+@[simp, scalar_tac_simp] theorem UScalar.bv_toNat_eq {ty : UScalarTy} (x : UScalar ty) :
   (UScalar.bv x).toNat  = x.val := by
   simp [val]
 
-@[simp] theorem U8.bv_toNat_eq (x : U8) : x.bv.toNat = x.val := by apply UScalar.bv_toNat_eq
-@[simp] theorem U16.bv_toNat_eq (x : U16) : x.bv.toNat = x.val := by apply UScalar.bv_toNat_eq
-@[simp] theorem U32.bv_toNat_eq (x : U32) : x.bv.toNat = x.val := by apply UScalar.bv_toNat_eq
-@[simp] theorem U64.bv_toNat_eq (x : U64) : x.bv.toNat = x.val := by apply UScalar.bv_toNat_eq
-@[simp] theorem U128.bv_toNat_eq (x : U128) : x.bv.toNat = x.val := by apply UScalar.bv_toNat_eq
-@[simp] theorem Usize.bv_toNat_eq (x : Usize) : x.bv.toNat = x.val := by apply UScalar.bv_toNat_eq
+@[simp, scalar_tac_simp] theorem U8.bv_toNat_eq (x : U8) : x.bv.toNat = x.val := by apply UScalar.bv_toNat_eq
+@[simp, scalar_tac_simp] theorem U16.bv_toNat_eq (x : U16) : x.bv.toNat = x.val := by apply UScalar.bv_toNat_eq
+@[simp, scalar_tac_simp] theorem U32.bv_toNat_eq (x : U32) : x.bv.toNat = x.val := by apply UScalar.bv_toNat_eq
+@[simp, scalar_tac_simp] theorem U64.bv_toNat_eq (x : U64) : x.bv.toNat = x.val := by apply UScalar.bv_toNat_eq
+@[simp, scalar_tac_simp] theorem U128.bv_toNat_eq (x : U128) : x.bv.toNat = x.val := by apply UScalar.bv_toNat_eq
+@[simp, scalar_tac_simp] theorem Usize.bv_toNat_eq (x : Usize) : x.bv.toNat = x.val := by apply UScalar.bv_toNat_eq
 
-@[simp] theorem IScalar.bv_toInt_eq {ty : IScalarTy} (x : IScalar ty) :
+@[simp, scalar_tac_simp] theorem IScalar.bv_toInt_eq {ty : IScalarTy} (x : IScalar ty) :
   (IScalar.bv x).toInt  = x.val := by
   simp [val]
 
-@[simp] theorem I8.bv_toInt_eq (x : I8) : x.bv.toInt = x.val := by apply IScalar.bv_toInt_eq
-@[simp] theorem I16.bv_toInt_eq (x : I16) : x.bv.toInt = x.val := by apply IScalar.bv_toInt_eq
-@[simp] theorem I32.bv_toInt_eq (x : I32) : x.bv.toInt = x.val := by apply IScalar.bv_toInt_eq
-@[simp] theorem I64.bv_toInt_eq (x : I64) : x.bv.toInt = x.val := by apply IScalar.bv_toInt_eq
-@[simp] theorem I128.bv_toInt_eq (x : I128) : x.bv.toInt = x.val := by apply IScalar.bv_toInt_eq
-@[simp] theorem Isize.bv_toInt_eq (x : Isize) : x.bv.toInt = x.val := by apply IScalar.bv_toInt_eq
+@[simp, scalar_tac_simp] theorem I8.bv_toInt_eq (x : I8) : x.bv.toInt = x.val := by apply IScalar.bv_toInt_eq
+@[simp, scalar_tac_simp] theorem I16.bv_toInt_eq (x : I16) : x.bv.toInt = x.val := by apply IScalar.bv_toInt_eq
+@[simp, scalar_tac_simp] theorem I32.bv_toInt_eq (x : I32) : x.bv.toInt = x.val := by apply IScalar.bv_toInt_eq
+@[simp, scalar_tac_simp] theorem I64.bv_toInt_eq (x : I64) : x.bv.toInt = x.val := by apply IScalar.bv_toInt_eq
+@[simp, scalar_tac_simp] theorem I128.bv_toInt_eq (x : I128) : x.bv.toInt = x.val := by apply IScalar.bv_toInt_eq
+@[simp, scalar_tac_simp] theorem Isize.bv_toInt_eq (x : Isize) : x.bv.toInt = x.val := by apply IScalar.bv_toInt_eq
 
 /-!
 Adding theorems to the `zify_simps` simplification set.
